@base <https://data.federatief.datastelsel.nl/lock-unlock/authentication/model/def/>.
@prefix : <https://data.kkg.kadaster.nl/authorisation/model#>.
@prefix owl: <http://www.w3.org/2002/07/owl#>.
@prefix rdf: <http://www.w3.org/1999/02/22-rdf-syntax-ns#>.
@prefix xsd: <http://www.w3.org/2001/XMLSchema#>.
@prefix rdfs: <http://www.w3.org/2000/01/rdf-schema#>.

: rdf:type owl:Ontology;
  owl:versionIRI :0.1.1.

:has_role rdf:type owl:ObjectProperty;
          rdfs:label "has_role";
          rdfs:subPropertyOf owl:topObjectProperty;
          rdfs:domain :User;
          rdfs:range :Role;
          rdfs:comment "Associates a user with one or more Roles, in accordance with section 2.1.4 of the paper by Jajodia et al. (2001)".

:Role rdf:type owl:Class;
      rdfs:label "Role";
      rdfs:comment "In line with the paper by Jajodia et al. (2001) this has been renamed from Persona to Role.".


:User rdf:type owl:Class;
      rdfs:label "User";
      rdfs:comment "A User is a natural person or autonomous system wishing to retrieve information from the dataset governed by the described authorisation policy.".
